\documentclass[12pt]{article}
\usepackage{lingmacros}
\usepackage{tree-dvips}
\begin{document}



\section{Problem 2}	
Exercise 2.3 on p. 42\\ 
Matlab Solution in file Problem2.m\\ \\
\textbf{Solution: {\LARGE $ \frac{-1}{\sqrt{10} * \sqrt{14}}$ }}\\

\noindent\rule{22cm}{0.4pt}
\\ \\
$V1 = <1, -3, 0> $\\
$V2 = <2, 1, 3> $\\

{\Large$cos(\theta) = \frac{ V1 \cdot V2}{\sqrt{1^2 + -3^2 + 0^2} * \sqrt{2^2 + 1^2 + 3^2}}$ }\\

\begin{enumerate}
\item[1. ] $cos(\theta) = \frac{ V1 \cdot V2}{\sqrt{1^2 + -3^2 + 0^2} * \sqrt{2^2 + 1^2 + 3^2}}$ 
\item[2. ] $V1 \cdot V2 = (1 * 2) + (1 * -3) + (0 * 3) = -1 $
\item[3. ] $\sqrt{1^2 + -3^2 + 0^2} = \sqrt{1 + 9} = \sqrt{10} $
\item[4. ] $ \sqrt{2^2 + 1^2 + 3^2} = \sqrt{4 + 1 + 9} = \sqrt{14}$
\item[5. ] $cos(\theta) = \frac{ V1 \cdot V2}{\sqrt{1^2 + -3^2 + 0^2} * \sqrt{2^2 + 1^2 + 3^2}} = \frac{-1}{\sqrt{10} * \sqrt{14}}$  
\end{enumerate}

{\LARGE $cos(\theta) = \frac{ V1 \cdot V2}{\sqrt{1^2 + -3^2 + 0^2} * \sqrt{2^2 + 1^2 + 3^2}} = \frac{-1}{\sqrt{10} * \sqrt{14}}$ }\\
\\ \\

\section{Problem 3}
Compute the Jacobian\\ \\
$x = u - v + w$\\
$y = u^2 - v^2 - w^2$\\
$z = u^3 + v$\\
\\
$Jacobian(u, v, w) = $\\

\[ \left( \begin{array}{ccc}
1 & -1 & 1 \\
2u & -2v & -2w \\
3u^2 & 1 & 0 \end{array} \right)\] 


\section{Problem 4}
Exercise 3.4 on pg. 76\\
Matlab Solution in file Problem4.m\\ \\


$M1 = $
\[ \left( \begin{array}{cccc}
2 & -1 & 1 & 0\\
1 & 3 & 1 & -1 \\
-2 & 1 & 0 & 1 \end{array} \right)\] 
\\ \\
$M2 = $
\[ \left( \begin{array}{cc}
1 & 2 \\
-2 & 0 \\
2 & -1 \\
1 & 1 \end{array} \right)\] 
\\ \\
$M1 \cdot M2 = $\\
\[ \left( \begin{array}{cc}
(2*1) + (-1*-2) + (1 * 2) + (0 * 1) & (2*2) + (-1*0) + (1 * -1) + (0 * 1)\\
(1*1) + (3*-2) + (1 * 2) + (-1 * 1) & (1*2) + (3*0) + (1 * -1) + (-1 * 1)\\
(-2*1) + (1*-2) + (0 * 2) + (1 * 1) & (-2*2) + (1*0) + (0 * -1) + (1 * 1)\end{array} \right)\] 
\\
{\Large $=$}
\\
\[ \left( \begin{array}{cc}
6 & 3\\
-4 & 0\\
-3 & -3\end{array} \right)\] 



\section{Problem 5}	
The textbook, Assignment 3.1 on pp. 78 - 79\\
Matlab Solutions in files evaluate.m and evaluate2.m\\

\section{Problem 6}
Let $z = 5 + 3i$ and $w = 2 - 4i$\\ \\

\begin{enumerate}
\item[(a)] $\bar{w} =$  {\Large$2 + 4i$ }\\
\item[(b)] $z + w = $  {\Large$7 - i$}\\  \\
$ 5 + 2 = 7$\\
$3i + -4i = -i $\\
$z + w = 7 - i$\\
\item[(c)]$z - w =$ {\Large$3 + 7i$}\\ \\
$5 - 2 = 3$\\
$3i - (-4i) = 7i$\\
$z - w = 3 + 7i$\\
\item[(d)] $zw = $ {\Large$22 - 14i$}\\ \\
$(5 + 3i)(2 - 4i) = $\\
$10 - 20i + 6i - 12i^2 = $\\
$10 - 14i + 12 = $\\
$22 - 14i$\\
\item[(e)] $z/w = $ {\Large$\frac{-1}{10} + \frac{13i}{10}$}\\ \\

{\Large $\frac{5 + 3i}{2 - 4i} = $\\ \\ \\
$\frac{(5 + 3i)(2 + 4i)}{(2 - 4i)(2 + 4i)} = $\\ \\ \\
$\frac{10 + 6i + 20i + 12i^2}{4 - 8i + 8i -16i^2} = $\\ \\ \\
$\frac{10 + 26i - 12}{20} = $\\ \\ \\
$\frac{-2 + 26i}{20} = $\\ \\ \\
$\frac{-1}{10} + \frac{13i}{10}$\\  \\ \\}
\end{enumerate}

\section{Problem 7}
\textit{Prove that}
$$\sin^3(\theta) = \frac{3}{4} sin(\theta) - \frac{1}{4}sin(3\theta)$$

\begin{enumerate}
{\Large
\item[1. ] $sin^3(\theta) = (\frac{e^{i\theta}-e^{-i\theta}}{2i})^3$
\item[2. ]  \hspace{7ex} $ = \frac{(e^{i\theta} - e^{-i\theta})^3}{8i^3}$
\item[3. ]  \hspace{7ex} $ = -\frac{1}{8i}((e^{i\theta})^3 - 3(e^{i\theta})^2(e^{-i\theta})
+ 3(e^{i\theta})(e^{-i\theta})^2 - (e^{-i\theta})^3)$
\item[4. ] \hspace{7ex} $ = -\frac{1}{8i}(e^{3i\theta} - 3e^{i\theta} 
+ 3e^{-i\theta} - e^{-3i\theta})$
\item[5. ] \hspace{7ex} $ = \frac{3}{4}(\frac{e^{i\theta} - e^{-i\theta}}{2i}) - 
\frac{1}{4}(\frac{e^{3i\theta} - e^{-3i\theta}}{2i})$
\item[6. ] \hspace{7ex} $ = \frac{3 sin \theta - sin (3\theta)}{4}$
\item[7. ] \hspace{7ex} $ = \frac{3}{4} sin(\theta) - \frac{1}{4}sin(3\theta)$
}
\end{enumerate}
\bibliographystyle{abbrv}
\bibliography{main}

\end{document}
This is never printed